Properties of renamings

HigherRankedSyntax/HigherRankedSyntax/Renaming.lean
@@ -7,18 +7,15 @@ infix:25 " →ʳ " => Renaming
 
 namespace Renaming
 
-@[reducible, simp]
 def id {γ} : γ →ʳ γ := fun {{_}} x => x
 
 notation "𝟙ʳ" => Renaming.id
 
-@[simp]
 def comp {γ δ η} (g : δ →ʳ η) (f : γ →ʳ δ) : γ →ʳ η :=
   fun {{_}} x => g (f x)
 
 infixr:90 " ∘ʳ " => Renaming.comp
 
-@[reducible]
 def extend {γ δ} (f : γ →ʳ δ) (η) : γ ⊕ η →ʳ δ ⊕ η
 | _, .varLeft x => .varLeft (f x)
 | _, .varRight y => .varRight y
@@ -31,10 +28,26 @@ def extend_id {γ η} : 𝟙ʳ ⇑ʳ η = @id (γ ⊕ η) := by
 
 def extend_comp {γ δ η θ} {g : δ →ʳ η} {f : γ →ʳ δ}:
   (g ∘ʳ f) ⇑ʳ θ = (g ⇑ʳ θ) ∘ʳ (f ⇑ʳ θ) := by
-  funext α x
+  funext _ x
   cases x <;> rfl
 
+@[reducible]
 def act {γ δ} (f : γ →ʳ δ) : Expr γ → Expr δ
   | x ◃ ts => f x ◃ (fun y => act (f ⇑ʳ _) (ts y))
+
+notation:60 "⟦" f "⟧ʳ " e:61 => Renaming.act f e
+
+theorem act_comp {γ} {e : Expr γ} :
+  ∀ {δ η} {f : γ →ʳ δ} {g : δ →ʳ η}, ⟦ g ∘ʳ f ⟧ʳ e = ⟦ g ⟧ʳ (⟦ f ⟧ʳ e) := by
+  induction e
+  case apply ih =>
+    intros
+    simp [comp, extend_comp]
+    funext
+    apply ih
+
+theorem comp_assoc {γ δ η θ} {f : γ →ʳ δ} {g : δ →ʳ η} {h : η →ʳ θ} :
+  (h ∘ʳ g) ∘ʳ f = h ∘ʳ (g ∘ʳ f) := by rfl
+
 
 end Renaming
