HigherRankedSyntax/HigherRankedSyntax/Syntax.lean
@@ -31,20 +31,6 @@ inductive Var : Arity → Shape → Type where
 | varLeft : ∀ {α γ δ}, Var α γ → Var α (γ ⊕ δ)
 | varRight : ∀ {α γ δ}, Var α δ → Var α (γ ⊕ δ)
 
-theorem Shape.rank_lt {γ δ} (x : Var γ δ) : γ.rank < δ.rank := by
-  induction x
-  case varHere => apply Nat.lt_add_of_pos_left Nat.zero_lt_one
-  case varLeft η β y ih =>
-    simp [Shape.rank]
-    calc
-      rank γ < 1 + rank γ            := by apply Nat.lt_add_of_pos_left Nat.zero_lt_one
-      _      < 1 + max η.rank β.rank := by apply Nat.add_lt_add_iff_left.2 ; sorry
-  case varRight η β y ih =>
-    simp [Shape.rank]
-    calc
-      rank γ < 1 + rank γ            := by apply Nat.lt_add_of_pos_left Nat.zero_lt_one
-      _      < 1 + max η.rank β.rank := by apply Nat.add_lt_add_iff_left.2 ; sorry
-
 inductive Expr : Shape → Type where
 | apply : ∀ {α γ}, Var α γ → (∀ {β}, Var β α → Expr (γ ⊕ β)) → Expr γ
 
